theories/memory.v
@@ -1,0 +1,112 @@
+(** a typeclass for a Wasm memory *)
+(* (C) J. Pichon - see LICENSE.txt *)
+
+Require Import BinNat.
+Require Import bytes.
+From mathcomp Require Import ssreflect ssrbool ssrfun eqtype.
+
+Module Memory.
+
+Definition mem_make_t Mem_t := byte -> N -> Mem_t.
+Definition mem_length_t Mem_t := Mem_t -> N.
+Definition mem_grow_t Mem_t := N -> Mem_t -> Mem_t.
+Definition mem_lookup_t Mem_t := N -> Mem_t -> option byte.
+Definition mem_update_t Mem_t := N -> byte -> Mem_t -> option Mem_t.
+
+Definition mem_ax_lookup_out_of_bounds
+  (Mem_t : Type)
+  (mem_make : mem_make_t Mem_t)
+  (mem_length : mem_length_t Mem_t)
+  (mem_grow : mem_grow_t Mem_t)
+  (mem_lookup : mem_lookup_t Mem_t)
+  (mem_update : mem_update_t Mem_t) :=
+  forall mem i, N.ge i (mem_length mem) -> mem_lookup i mem = None.
+
+Definition mem_ax_lookup_make
+  (Mem_t : Type)
+  (mem_make : mem_make_t Mem_t)
+  (mem_length : mem_length_t Mem_t)
+  (mem_grow : mem_grow_t Mem_t)
+  (mem_lookup : mem_lookup_t Mem_t)
+  (mem_update : mem_update_t Mem_t) :=
+  forall i len b, N.lt i len -> mem_lookup i (mem_make b len) = Some b.
+
+Definition mem_ax_lookup_update
+  (Mem_t : Type)
+  (mem_make : mem_make_t Mem_t)
+  (mem_length : mem_length_t Mem_t)
+  (mem_grow : mem_grow_t Mem_t)
+  (mem_lookup : mem_lookup_t Mem_t)
+  (mem_update : mem_update_t Mem_t) :=
+  forall mem mem' i b, N.lt i (mem_length mem) -> Some mem' = mem_update i b mem -> mem_lookup i mem' = Some b.
+
+Definition mem_ax_lookup_skip
+  (Mem_t : Type)
+  (mem_make : mem_make_t Mem_t)
+  (mem_length : mem_length_t Mem_t)
+  (mem_grow : mem_grow_t Mem_t)
+  (mem_lookup : mem_lookup_t Mem_t)
+  (mem_update : mem_update_t Mem_t) :=
+  forall mem mem' i i' b, i <> i' -> Some mem' = mem_update i' b mem -> mem_lookup i mem' = mem_lookup i mem.
+
+Definition mem_ax_length_constant_update
+  (Mem_t : Type)
+  (mem_make : mem_make_t Mem_t)
+  (mem_length : mem_length_t Mem_t)
+  (mem_grow : mem_grow_t Mem_t)
+  (mem_lookup : mem_lookup_t Mem_t)
+  (mem_update : mem_update_t Mem_t) :=
+  forall i b mem mem', Some mem' = mem_update i b mem -> mem_length mem' = mem_length mem.
+
+Set Implicit Arguments.
+Unset Strict Implicit.
+Unset Printing Implicit Defensive.
+
+Section ClassDef.
+
+Record mixin_of (Mem_t : Type) : Type := Mixin {
+  mem_make : byte -> N -> Mem_t;
+  mem_length : Mem_t -> N;
+  mem_grow : mem_grow_t Mem_t;
+  mem_lookup : mem_lookup_t Mem_t;
+  mem_update : N -> byte -> Mem_t -> option Mem_t;
+  _ : mem_ax_lookup_out_of_bounds Mem_t mem_make mem_length mem_grow mem_lookup mem_update;
+  _ : mem_ax_lookup_make Mem_t mem_make mem_length mem_grow mem_lookup mem_update;
+  _ : mem_ax_lookup_update Mem_t mem_make mem_length mem_grow mem_lookup mem_update;
+  _ : mem_ax_lookup_skip Mem_t mem_make mem_length mem_grow mem_lookup mem_update;
+  _ : mem_ax_length_constant_update Mem_t mem_make mem_length mem_grow mem_lookup mem_update;
+}.
+
+Set Primitive Projections.
+Record class_of (T : Type) : Type := Class {base : Equality.mixin_of T; mixin : mixin_of T}.
+Unset Primitive Projections.
+Local Coercion base : class_of >->  Equality.class_of.
+
+Structure type : Type := Pack {sort; _ : class_of sort; }.
+Local Coercion sort : type >-> Sortclass.
+
+Variables (T : Type) (cT : type).
+Definition class := let: Pack _ c as cT' := cT return class_of cT' in c.
+Definition clone c of phant_id class c := @Pack T c.
+Let xT := let: Pack T _ := cT in T.
+Notation xclass := (class : class_of xT).
+
+Definition pack m :=
+  fun b bT & phant_id (Equality.class bT) b => Pack (@Class T b m).
+
+Definition eqType := @Equality.Pack cT xclass.
+
+End ClassDef.
+
+Module Import Exports.
+Coercion base : class_of >-> Equality.class_of.
+Coercion sort : type >-> Sortclass.
+Coercion eqType : type >-> Equality.type.
+Canonical eqType.
+Notation memoryType := type.
+Notation memoryMixin := mixin_of.
+Notation MemoryType T m := (@pack T m _ _ id).
+
+End Exports.
+
+End Memory.
