theories/memory_list.v
@@ -1,0 +1,173 @@
+(** an implementation of Wasm memory based on a list *)
+(* (C) J. Pichon - see LICENSE.txt *)
+
+From mathcomp Require Import ssreflect ssrbool eqtype seq.
+Require Import BinNat Lia.
+From Wasm Require Import numerics bytes memory.
+
+Record memory_list : Type := {
+  ml_init : byte;
+  ml_data : list byte;
+}.
+
+Definition mem_make : Memory.mem_make_t memory_list :=
+  fun v len => {| ml_init := v; ml_data := List.repeat v (N.to_nat len) |}.
+
+Definition mem_length : Memory.mem_length_t memory_list :=
+    fun ml => N.of_nat (List.length ml.(ml_data)).
+
+Definition mem_grow : Memory.mem_grow_t memory_list :=
+  fun len_delta ml =>
+    {|
+      ml_init := ml.(ml_init);
+      ml_data := ml.(ml_data) ++ List.repeat ml.(ml_init) (N.to_nat len_delta)
+    |}.
+
+Definition mem_lookup : Memory.mem_lookup_t memory_list :=
+  fun i ml => List.nth_error ml.(ml_data) (N.to_nat i).
+
+Definition mem_update : Memory.mem_update_t memory_list :=
+  fun i v ml =>
+    if N.ltb i (N.of_nat (List.length ml.(ml_data)))
+    then Some {| ml_init := ml.(ml_init);
+                ml_data := take (N.to_nat i) ml.(ml_data) ++ [::v] ++ drop (N.to_nat i+1) ml.(ml_data) |}
+    else None.
+
+Lemma memory_list_ax_lookup_out_of_bounds :
+  Memory.mem_ax_lookup_out_of_bounds memory_list mem_make mem_length mem_grow mem_lookup mem_update.
+Proof.
+move => mem i.
+rewrite /mem_length /mem_lookup.
+move => H.
+apply (List.nth_error_None mem.(ml_data) (N.to_nat i)).
+apply N.ge_le in H.
+move: H.
+set x := (length (ml_data mem)).
+move => H.
+lia.
+Qed.
+  
+Lemma nth_repeat :
+forall A b i len, i < len ->
+@List.nth_error A (List.repeat b len) i = Some b.
+Proof.
+move => A b.
+elim => [|i].
+{ case => [|len]; first by lia.
+  by move => _. }
+{ move => IH len.
+  case: len => [|len'].
+  { move => Hctr.
+    exfalso.
+    lia. }
+  { move => Hlen /=.
+    apply: IH.
+    lia. } }
+Qed.
+  
+Lemma lookup_split : forall A (l : list A) i b,
+  i < List.length l ->
+  List.nth_error (take i l ++ b :: drop (i+1) l) i = Some b.
+Proof.
+move => A.
+elim => [|x l].
+{ move => i b /= Hlen.
+  exfalso.
+  lia. }
+{ move => IH.
+  case => [|i]; first by reflexivity.
+  move => b /= Hlen.
+  have Hlen': i < length l by lia.
+  by apply: IH. }
+Qed.
+  
+Lemma bar : forall A n n' (l : list A) v,
+  n <> n' -> n' < List.length l ->
+  List.nth_error (take n' l ++ v :: drop (n' + 1) l) n =
+  List.nth_error l n.
+Proof.
+(* TODO *)
+Admitted.
+
+Lemma split_preserves_length : forall A i b (l : list A),
+  i < List.length l ->
+  List.length (take i l ++ b :: drop (i + 1) l) = List.length l.
+Proof.
+Admitted.
+
+Lemma memory_list_ax_lookup_make : Memory.mem_ax_lookup_make memory_list mem_make mem_length mem_grow mem_lookup mem_update.
+Proof.
+move => i len b mem.
+apply: nth_repeat.
+lia.
+Qed.
+
+Lemma memory_list_ax_lookup_update :
+  Memory.mem_ax_lookup_update memory_list mem_make mem_length mem_grow mem_lookup mem_update.
+Proof.
+move => mem mem' i b H H0.
+rewrite /mem_update in H0.
+apply N.ltb_lt in H.
+rewrite /mem_length in H.
+rewrite H in H0.
+case: mem' H0 => init_ data_ [Hinit Hdata].
+rewrite Hinit Hdata /= {init_ data_ Hinit Hdata}.
+set nn := N.to_nat i.
+have Hx: nn < length (ml_data mem).
+apply N.ltb_lt in H.
+lia.
+by apply: lookup_split.
+Qed.
+
+Lemma memory_list_ax_lookup_skip :
+  Memory.mem_ax_lookup_skip memory_list mem_make mem_length mem_grow mem_lookup mem_update.
+Proof.
+move => mem mem' i i' b Hii' H0.
+case: mem' H0 => init_ data_.
+rewrite /mem_update /mem_lookup.
+case_eq (N.ltb i' (N.of_nat (length (ml_data mem)))); last by discriminate.
+move => Hlen [Hinit Hdata] /=.
+rewrite Hdata => {Hdata}.
+apply: bar.
+lia.
+apply N.ltb_lt in Hlen.
+lia.
+Qed.
+
+Lemma memory_list_ax_length_constant_update :
+  Memory.mem_ax_length_constant_update memory_list mem_make mem_length mem_grow mem_lookup mem_update.
+Proof.
+move => i b [dv_init1 dv_list1] [dv_init2 dv_list2].
+rewrite /mem_update /mem_length /=.
+case_eq (N.ltb i (N.of_nat (length dv_list1))); last by discriminate.
+move => Hlen [Hinit Hlist].
+apply N.ltb_lt in Hlen.
+rewrite Hlist.
+f_equal.
+apply: (split_preserves_length _ (N.to_nat i) b dv_list1).
+lia.
+Qed.
+
+
+Require Import bytes common.
+
+Definition memory_list_eq_dec : forall (i1 i2 : memory_list), {i1 = i2} + {i1 <> i2}.
+Proof. decidable_equality. Defined.
+
+Definition memory_list_eqb i1 i2 : bool := memory_list_eq_dec i1 i2.
+
+Definition eqmemory_listP : Equality.axiom memory_list_eqb :=
+  eq_dec_Equality_axiom memory_list_eq_dec.
+
+Canonical Structure memory_list_eqMixin := EqMixin eqmemory_listP.
+Canonical Structure memory_list_eqType := Eval hnf in EqType memory_list memory_list_eqMixin.
+
+Definition list_memoryMixin :=
+  Memory.Mixin
+    memory_list_ax_lookup_out_of_bounds
+    memory_list_ax_lookup_make
+    memory_list_ax_lookup_update
+    memory_list_ax_lookup_skip
+    memory_list_ax_length_constant_update.
+Definition list_memoryClass := Memory.Class memory_list_eqMixin list_memoryMixin.
+Canonical list_memoryType := @Memory.Pack memory_list list_memoryClass.
